Start verifying stuff

theories/FileSystem.v
@@ -3,7 +3,10 @@ From FreeSpec Require Import Core.
 
 Generalizable All Variables.
 
+(** * Definition  *)
+
 Axiom file_descriptor : Type.
+Axiom fd_eq_dec : forall (fd1 fd2 : file_descriptor), { fd1 = fd2 } + { ~ (fd1 = fd2) }.
 
 Inductive FILESYSTEM : interface :=
 | Open (path : string) : FILESYSTEM file_descriptor
@@ -22,3 +25,96 @@ Definition is_file `{Provide ix FILESYSTEM} (path : string) : impure ix bool :=
 
 Definition read `{Provide ix FILESYSTEM} (fd : file_descriptor) : impure ix string :=
   request (Read fd).
+
+(** * Contracts *)
+
+Definition fd_set : Type := file_descriptor -> bool.
+
+Definition add_fd (ω : fd_set) (fd : file_descriptor) : fd_set :=
+  fun (fd' : file_descriptor) => if fd_eq_dec fd fd' then true else ω fd'.
+
+Definition del_fd (ω : fd_set) (fd : file_descriptor) : fd_set :=
+  fun (fd' : file_descriptor) => if fd_eq_dec fd fd' then false else ω fd'.
+
+Definition member (ω : fd_set) (fd : file_descriptor) : Prop :=
+  ω fd = true.
+
+Definition absent (ω : fd_set) (fd : file_descriptor) : Prop :=
+  ω fd = false.
+
+Lemma member_not_absent (ω : fd_set) (fd : file_descriptor)
+  : member ω fd -> ~ absent ω fd.
+
+Proof.
+  unfold member, absent.
+  intros m a.
+  now rewrite m in a.
+Qed.
+
+Hint Resolve member_not_absent.
+
+Lemma absent_not_member (ω : fd_set) (fd : file_descriptor)
+  : absent ω fd -> ~ member ω fd.
+
+Proof.
+  unfold member, absent.
+  intros a m.
+  now rewrite m in a.
+Qed.
+
+Hint Resolve absent_not_member.
+
+Lemma member_add_fd (ω : fd_set) (fd : file_descriptor) : member (add_fd ω fd) fd.
+
+Proof.
+  unfold member, add_fd.
+  destruct fd_eq_dec; auto.
+Qed.
+
+Hint Resolve member_add_fd.
+
+Definition fd_set_update (ω : fd_set) (a : Type) (e : FILESYSTEM a) (x : a) : fd_set :=
+  match e, x with
+  | Open _, fd =>
+    add_fd ω fd
+  | Close fd, _ =>
+    del_fd ω fd
+  | Read _, _ =>
+    ω
+  | IsFile _, _ =>
+    ω
+  end.
+
+Inductive fd_set_caller_obligation (ω : fd_set) : forall (a : Type), FILESYSTEM a -> Prop :=
+| fd_set_open_caller (p : string)
+  : fd_set_caller_obligation ω file_descriptor (Open p)
+| fd_set_read_caller (fd : file_descriptor) (is_member : member ω fd)
+  : fd_set_caller_obligation ω string (Read fd)
+| fd_set_close_caller (fd : file_descriptor) (is_member : member ω fd)
+  : fd_set_caller_obligation ω unit (Close fd)
+| fd_set_is_file_caller (p : string)
+  : fd_set_caller_obligation ω bool (IsFile p).
+
+Hint Constructors fd_set_caller_obligation.
+
+Inductive fd_set_callee_obligation (ω : fd_set) : forall (a : Type), FILESYSTEM a -> a -> Prop :=
+| fd_set_open_callee (p : string) (fd : file_descriptor) (is_absent : absent ω fd)
+  : fd_set_callee_obligation ω file_descriptor (Open p) fd
+| fd_set_read_callee (fd : file_descriptor) (s : string)
+  : fd_set_callee_obligation ω string (Read fd) s
+| fd_set_close_callee (fd : file_descriptor) (t : unit)
+  : fd_set_callee_obligation ω unit (Close fd) t
+| fd_set_is_file_callee (p : string) (b : bool)
+  : fd_set_callee_obligation ω bool (IsFile p) b.
+
+Hint Constructors fd_set_callee_obligation.
+
+Definition fd_set_specs : specs FILESYSTEM fd_set :=
+  {| witness_update := fd_set_update
+   ; requirements := fd_set_caller_obligation
+   ; promises := fd_set_callee_obligation
+  |}.
+
+Definition fd_set_preserving {a} `{Provide ix FILESYSTEM} (p : impure ix a) :=
+  forall (ω ω' : fd_set) (x : a),
+    trustworthy_run fd_set_specs p ω ω' x -> forall fd, ω fd = ω' fd.
