theories/HTTP.v
@@ -1,11 +1,8 @@
-From FreeSpec Require Import Core.
-From Praecia Require Import Parser URI FileSystem TCP.
+From Praecia Require Import Parser URI.
 
 Import ListNotations.
 #[local] Open Scope string_scope.
 #[local] Open Scope prelude_scope.
-
-Generalizable All Variables.
 
 Inductive request :=
 | Get (resource : uri).
@@ -37,45 +34,3 @@ Definition response_to_string (res : response) : string :=
 
 Definition http_request : parser request :=
   Get <$> (str "GET" *> whitespaces *> read_uri <* whitespaces <* str "HTTP/1.1").
-
-Definition sandbox (base : list directory_id) (req : uri) : uri :=
-  make_uri (List.app base (canonicalize (dirname req))) (filename req).
-
-(* TODO: add a notation in coq-prelude var (x : T) <- p in q *)
-Definition request_handler `{Provide ix FILESYSTEM}
-    (base : list directory_id) (req : request)
-  : impure ix response :=
-  match req with
-  | Get uri =>
-    do let path := uri_to_path (sandbox base uri) in
-       var isf <- is_file path in
-       if (isf : bool)
-       then do var fd <- open path in
-               var content <- (read fd <* close fd) in
-               pure (make_response success_OK content)
-            end
-       else pure (make_response client_error_NotFound "Resource not found.")
-    end
-  end.
-
-Definition tcp_handler `{Provide ix FILESYSTEM}
-    (base : list directory_id) (req : string)
-  : impure ix string :=
-  response_to_string <$> match parse http_request req with
-                         | inl _ => pure (make_response client_error_BadRequest "")
-                         | inr req => request_handler base req
-                         end.
-
-Definition http_server `{Provide ix FILESYSTEM, Provide ix TCP}
-  : impure ix unit :=
-  do var server <- new_tcp_socket "localhost:8000" in
-     listen_incoming_connection server;
-
-     var client <- accept_connection server in
-     var req <- read_socket client in
-     var res <- tcp_handler [Dirname "opt"; Dirname "praecia"] req in
-
-     write_socket client res;
-     close_socket client;
-     close_socket server
-  end.
