theories/Server.v
@@ -1,0 +1,126 @@
+From FreeSpec Require Import Core Core.Notations.
+From Praecia Require Import FileSystem TCP URI HTTP Parser.
+From Prelude Require Import Tactics.
+
+Import ListNotations.
+#[local] Open Scope string_scope.
+#[local] Open Scope prelude_scope.
+
+Generalizable All Variables.
+
+Definition sandbox (base : list directory_id) (req : uri) : uri :=
+  make_uri (List.app base (canonicalize (dirname req))) (filename req).
+
+Definition read_content `{Provide ix FILESYSTEM} (path : string)
+  : impure ix string :=
+  open path >>= fun fd => read fd <* close fd.
+
+(* TODO: add a notation in coq-prelude var (x : T) <- p in q *)
+Definition request_handler `{Provide ix FILESYSTEM}
+    (base : list directory_id) (req : request)
+  : impure ix response :=
+  match req with
+  | Get uri =>
+    do let path := uri_to_path (sandbox base uri) in
+       var isf <- is_file path in
+       if (isf : bool)
+       then make_response success_OK <$> read_content path
+       else pure (make_response client_error_NotFound "Resource not found.")
+    end
+  end.
+
+Definition tcp_handler `{Provide ix FILESYSTEM}
+    (base : list directory_id) (req : string)
+  : impure ix string :=
+  response_to_string <$> match parse http_request req with
+                         | inl _ => pure (make_response client_error_BadRequest "")
+                         | inr req => request_handler base req
+                         end.
+
+Definition http_server `{Provide ix FILESYSTEM, Provide ix TCP}
+  : impure ix unit :=
+  do var server <- new_tcp_socket "localhost:8000" in
+     listen_incoming_connection server;
+
+     var client <- accept_connection server in
+     var req <- read_socket client in
+     var res <- tcp_handler [Dirname "opt"; Dirname "praecia"] req in
+
+     write_socket client res;
+     close_socket client;
+     close_socket server
+  end.
+
+Lemma fd_set_trustworthy_read_content `{Provide ix FILESYSTEM} (ω : fd_set) (path : string)
+  : trustworthy_impure fd_set_specs ω (read_content path).
+
+Proof.
+  now prove_impure.
+Qed.
+
+Hint Resolve fd_set_trustworthy_read_content.
+
+Lemma fd_set_preserving_read_content `{Provide ix FILESYSTEM} (path : string)
+  : fd_set_preserving (read_content path).
+
+Proof.
+  intros ω ω' x run.
+  unroll_impure_run run.
+  intros fd'.
+  unfold add_fd, del_fd.
+  destruct fd_eq_dec; subst.
+  + now inversion prom; ssubst.
+  + reflexivity.
+Qed.
+
+#[local] Opaque read_content.
+
+Lemma fd_set_trustworthy_is_file `{Provide ix FILESYSTEM} (ω : fd_set) (path : string)
+  : trustworthy_impure fd_set_specs ω (is_file path).
+
+Proof.
+  now prove_impure.
+Qed.
+
+Hint Resolve fd_set_trustworthy_is_file.
+
+Lemma fd_set_preserving_is_file `{Provide ix FILESYSTEM} (path : string)
+  : fd_set_preserving (is_file path).
+
+Proof.
+  intros ω ω' x run.
+  now unroll_impure_run run.
+Qed.
+
+#[local] Opaque is_file.
+
+Lemma fd_set_trustworthy_request_handler `{Provide ix FILESYSTEM}
+    (base : list directory_id) (req : request) (ω : fd_set)
+  : trustworthy_impure fd_set_specs ω (request_handler base req).
+
+Proof.
+  destruct req.
+  prove_impure; auto.
+  unfold impure_map. (* FIXME: should be done by the [prove_impure] tactic *)
+  now prove_impure.
+Qed.
+
+Lemma fd_set_preserving_request_handler `{Provide ix FILESYSTEM}
+    (base : list directory_id) (req : request)
+  : fd_set_preserving (request_handler base req).
+
+Proof.
+  intros ω ω' x run fd.
+  destruct req.
+  unroll_impure_run run.
+  + unfold impure_map in run1. (* FIXME: should be done by unroll_impure_run tactic *)
+    unroll_impure_run run1.
+
+    apply fd_set_preserving_is_file in run0.
+    apply fd_set_preserving_read_content in run.
+
+    now transitivity (ω'' fd).
+  + now apply fd_set_preserving_is_file in run0.
+Qed.
+
+#[local] Opaque request_handler.
